\documentclass{article}

\begin{document}

Chapter1: Induction.

1. Prove that
$1^2 + 2^2 + 3^2\ldots{} + n^2 = \frac{n(n+1)(2n+1)}{6}$ \\

2. Prove that
$1^3 + 2^3 + 3^3\ldots{} + n^3 = (1 + 2 + 3 + \ldots{} + n)^2$ \\

3. Prove that
$x^n-y^n = (x - y)(x^{n-1} + x^{n-2}y + \ldots{} + xy^{n-2} + y^{n-1})$ \\

4. Porve that
$1\cdot2 + 2\cdot3 + 3\cdot4 + \ldots{} + n(n+1) = \frac{n(n+1)(n+2)}{3}$ \\

5. Prove that
$1 + 3 + 5 + \ldots{} + (2n-1) = n^2 $ \\

6. Prove that
$\frac{1}{1\cdot2} + \frac{1}{2\cdot3}  + \frac{1}{3\cdot4} \ldots{} + \frac{1}{n(n+1)} = \frac{n}{n+1} $ \\

7. Take the Fibonacci Sequence where
$F_1 = 1,F_2 = 1, F_3 = 2$ and subsquently $F_n = F_{n-1} + F_{n-2}$. Prove that $F_1 + F_2 + F_3 + \ldots + F_n = F_{n+2} - 1$ \\

8. Prove that
$F_1 + F_3 + F_5 + \ldots + F_{2n-1} = F_{2n}$ \\

9. Prove that
$F_2 + F_4 + F_6 + \ldots + F_{2n} = F_{2n + 1} - 1$ \\

10. Prove that
$F_{n+1}^2 - F_nF_{n+2} =  (- 1)^n$ \\

11. Prove that
$F_1F_2 + F_2F_3 + F_3F_4 + \ldots + F_{2n - 1}F_{2n} = F_{2n}^2$\\

12. Prove that
$F_1F_2 + F_2F_3 + F_3F_4 + \ldots + F_{2n}F_{2n+1} = F_{2n+1}^2 -1$\\

13. Take the Lucas Numbers $L_n$ which are the difined by the equations $L_1 =1$ and $L_n = F_{n+1} + F_{n-1}$ for each $ n \geq 2$. Prove that $L_n = L_{n-1} + L_{n-2} \quad (n \geq 3)$ \\

14. What is wrong with the following arguement:
TODO

15. Prove that
$F_{2n} = F_nL_n$\\

16. Prove that
$L_1 + 2L_2 + 4l_3 + 8L_4 \ldots + 2^{n-1}L_n = 2^nF_{n+1} - 1$\\

17. Prove that
$n(n^2-1)(3n+2)$ is divisible by 24 for each positive integer

18. Prove that if $n$ is an odd positive integer, then $x^n + y^n \mid x+y$
\end{document}